Suppose we have a GLWE ciphertext $C$ and a new plaintext polynomial $\Lambda$ as follows: 


$C = \textsf{GLWE}_{S, \sigma}(\Delta M) = ( A_1, A_2, \gap{$\cdots$}, A_{k-1}, B) \in \mathcal{R}_{\langle n,q \rangle}^{k + 1}$

$\Lambda$: a new plaintext polynomial

$\Delta \Lambda$: a $\Delta$-scaled new plaintext polynomial

$ $

\noindent Let's define the following TFHE ciphertext-to-plaintext addition operation: 

$C + \Delta\Lambda = ( A_1, \text{ } A_2, \gap{$\cdots$}, A_{k-1}, \text{ } B + \Delta \Lambda)$

$ $

\noindent Then, the following is true:

\begin{tcolorbox}[title={\textbf{\tboxlabel{\ref*{sec:glwe-add-plain}} GLWE Homomorphic Addition with a Plaintext}}]
$\textsf{GLWE}_{S, \sigma}(\Delta M) + \Delta\Lambda $

$=  (\{A_i^{\langle 1 \rangle}\}_{i=0}^{k-1}, \text{ } B^{\langle 1 \rangle}) + \Delta\Lambda$

$=  (\{A_i^{\langle 1 \rangle}\}_{i=0}^{k-1}, \text{ } B^{\langle 1 \rangle} + \Delta\Lambda)$

$= \textsf{GLWE}_{S, \sigma}(\Delta (M + \Lambda) )$
\end{tcolorbox}


This means that a plaintext polynomial to a TFHE ciphertext and decrypting it gives the same result as adding two original plaintexts. 




\begin{myproof}

\begin{enumerate}
\item Since $B = \sum\limits_{i=0}^{k-1}{(A_i \cdot S_i)} + \Delta \cdot M + E$,

$B + \Delta \cdot \Lambda = \sum\limits_{i=0}^{k-1}{(A_i \cdot S_i)} + \Delta \cdot M + E + \Delta \cdot \Lambda = \sum\limits_{i=0}^{k-1}{(A_i \cdot S_i)} + \Delta \cdot (M + \Lambda) + E$  \\

This means that $(A_1, A_2, ... \text{ } A_{k-1}
, B + \Delta \Lambda)$ form the ciphertext $\textsf{GLWE}_{S, \sigma}(\Delta (\Lambda + M))$
\item Thus, \\
$\textsf{GLWE}_{S, \sigma}(\Delta M) + \Delta\Lambda$ \\
$ = (A_0, \text { } A_1, ... \text{ } A_{k-1}, \text { } B + \Delta \Lambda)$ \\
$ = (\{A_i^{\langle 1 \rangle}\}_{i=0}^{k-1}, \text { } B + \Delta \Lambda)$ \\
$= \textsf{GLWE}_{S, \sigma}(\Delta (M + \Lambda))$

%\begin{flushright}
%\qedsymbol{} 
%\end{flushright}
\end{enumerate}

\end{myproof}


\subsection{Discussion}

\para{Noise Growth: } Note that after decryption, the original ciphertext $C +\Lambda$'s noise $E$ stays the same as before. This means that ciphertext-to-plaintext multiplication does not increase the noise level.